Blake2s: towards better testing for the stateful code

code/blake2/Hacl.Test.Blake2s.fst
@@ -1,87 +1,81 @@
 module Hacl.Test.Blake2s
 
-#reset-options "--z3rlimit 100 --max_fuel 0 --lax"
-
 open FStar.HyperStack.All
 open FStar.Mul
+
+open LowStar.Buffer
+
 open Lib.IntTypes
-open Lib.RawIntTypes
 open Lib.Buffer
+open Lib.Print
+open Hacl.Blake2s
 
-//
-// Test 1
-//
 
-// inline_for_extraction let test1_plaintext_len = size 3
-// inline_for_extraction let test1_plaintext : list uint8 = [
-//   u8 0x61; u8 0x62; u8 0x63
-// ]
+val test_blake2s:
+    msg_len:size_t
+  -> msg:lbytes (size_v msg_len)
+  -> key_len:size_t{v key_len <= 32 /\ (if v key_len = 0 then v msg_len < pow2 64 else v msg_len + 64 < pow2 64)}
+  -> key:lbytes (size_v key_len)
+  -> expected_len:size_t{1 <= v expected_len /\ v expected_len <= 32}
+  -> expected:lbytes (size_v expected_len)
+  -> Stack unit
+    (requires fun h ->
+      live h msg /\ live h expected /\ live h key)
+    (ensures  fun h0 r h1 -> True)
 
-// inline_for_extraction let test1_expected_len = size 32
-// inline_for_extraction let test1_expected :  list uint8 = [
-//   u8 0x50; u8 0x8C; u8 0x5E; u8 0x8C; u8 0x32; u8 0x7C; u8 0x14; u8 0xE2;
-//   u8 0xE1; u8 0xA7; u8 0x2B; u8 0xA3; u8 0x4E; u8 0xEB; u8 0x45; u8 0x2F;
-//   u8 0x37; u8 0x45; u8 0x8B; u8 0x20; u8 0x9E; u8 0xD6; u8 0x3A; u8 0x29;
-//   u8 0x4D; u8 0x99; u8 0x9B; u8 0x4C; u8 0x86; u8 0x67; u8 0x59; u8 0x82
-// ]
+let test_blake2s msg_len msg key_len key expected_len expected =
+  push_frame();
+  let result = create #_ #(v expected_len) expected_len (u8 0) in
+  blake2s result msg msg_len key key_len expected_len;
+  print_compare_display expected_len result expected;
+  pop_frame()
 
-// inline_for_extraction let empty : list uint8 = []
+
+///
+/// Test 1
+///
+
+inline_for_extraction let test1_size_plaintext = 3
+let test1_plaintext: b:lbytes test1_size_plaintext{ recallable b } =
+  [@ inline_let]
+  let l:list uint8 =
+    normalize_term (List.Tot.map u8
+    [0x61; 0x62; 0x63])
+  in
+  assert_norm (List.Tot.length l == 3);
+  createL_global l
+
+inline_for_extraction let test1_size_key = 0
+let test1_key: b:lbytes test1_size_key{ recallable b } =
+  let open Lib.RawIntTypes in
+  [@ inline_let]
+  let l:list uint8 =
+    normalize_term (List.Tot.map u8 []) in
+  assert_norm (List.Tot.length l == 0); admit();
+  createL_global l
+
+inline_for_extraction let test1_size_expected = 32
+let test1_expected: b:lbytes test1_size_expected{ recallable b } =
+  [@ inline_let]
+  let l:list uint8 =
+    normalize_term (List.Tot.map u8
+    [ 0x50; 0x8C; 0x5E; 0x8C; 0x32; 0x7C; 0x14; 0xE2;
+      0xE1; 0xA7; 0x2B; 0xA3; 0x4E; 0xEB; 0x45; 0x2F;
+      0x37; 0x45; 0x8B; 0x20; 0x9E; 0xD6; 0x3A; 0x29;
+      0x4D; 0x99; 0x9B; 0x4C; 0x86; 0x67; 0x59; 0x82])
+  in
+  assert_norm (List.Tot.length l == 32);
+  createL_global l
 
 //
 // Main
 //
 
-val main: unit -> Stack C.exit_code (requires (fun h -> True)) (ensures (fun h0 _ h1 -> True))
+val main: unit -> St C.exit_code
 let main () =
-
-  let test1_plaintext_len = size 3 in
-  let test1_expected_len = size 32 in
-  let test1_empty_len = size 0 in
-
-  let test1_plaintext : buffer uint8 =
-    createL [
-      u8 0x61; u8 0x62; u8 0x63
-    ] in
-  let test1_expected : buffer uint8 =
-    createL [
-      u8 0x50; u8 0x8C; u8 0x5E; u8 0x8C; u8 0x32; u8 0x7C; u8 0x14; u8 0xE2;
-      u8 0xE1; u8 0xA7; u8 0x2B; u8 0xA3; u8 0x4E; u8 0xEB; u8 0x45; u8 0x2F;
-      u8 0x37; u8 0x45; u8 0x8B; u8 0x20; u8 0x9E; u8 0xD6; u8 0x3A; u8 0x29;
-      u8 0x4D; u8 0x99; u8 0x9B; u8 0x4C; u8 0x86; u8 0x67; u8 0x59; u8 0x82
-    ] in
-  let empty : buffer uint8 = createL [] in
-  C.String.print (C.String.of_literal "\nTEST 1\n");
-  let test1_result : buffer uint8 = create #uint8 #32 (size 32) (u8 0) in
-
-  Hacl.Blake2s.blake2s test1_result test1_plaintext test1_plaintext_len empty test1_empty_len (size 32);
-  Lib.Print.print_compare_display test1_expected_len test1_result test1_expected;
-
-  (* let test2_plaintext_len = size 1 in *)
-  (* let test2_key_len = size 32 in *)
-  (* let test2_expected_len = size 32 in *)
-
-  (* let test2_plaintext : lbuffer uint8 (size_v test2_plaintext_len) = *)
-  (*   createL [ u8 0x00 ] in *)
-  (* let test2_key : lbuffer uint8 (size_v test2_expected_len) = *)
-  (*   createL [ *)
-  (*     u8 0x00; u8 0x01; u8 0x02; u8 0x03; u8 0x04; u8 0x05; u8 0x06; u8 0x07; *)
-  (*     u8 0x08; u8 0x09; u8 0x0a; u8 0x0b; u8 0x0c; u8 0x0d; u8 0x0e; u8 0x0f; *)
-  (*     u8 0x10; u8 0x11; u8 0x12; u8 0x13; u8 0x14; u8 0x15; u8 0x16; u8 0x17; *)
-  (*     u8 0x18; u8 0x19; u8 0x1a; u8 0x1b; u8 0x1c; u8 0x1d; u8 0x1e; u8 0x1f *)
-  (*   ] in *)
-  (* let test2_expected : lbuffer uint8 (size_v test2_key_len) = *)
-  (*   createL [ *)
-  (*     u8 0x40; u8 0xd1; u8 0x5f; u8 0xee; u8 0x7c; u8 0x32; u8 0x88; u8 0x30; *)
-  (*     u8 0x16; u8 0x6a; u8 0xc3; u8 0xf9; u8 0x18; u8 0x65; u8 0x0f; u8 0x80; *)
-  (*     u8 0x7e; u8 0x7e; u8 0x01; u8 0xe1; u8 0x77; u8 0x25; u8 0x8c; u8 0xdc; *)
-  (*     u8 0x0a; u8 0x39; u8 0xb1; u8 0x1f; u8 0x59; u8 0x80; u8 0x66; u8 0xf1 *)
-  (*   ] in *)
-
-  (* C.String.print (C.String.of_literal "\nTEST 2\n"); *)
-  (* let test2_result : lbuffer uint8 (size_v test2_expected_len) = create #uint8 (size 32) (u8 0) in *)
-  (* Hacl.Impl.Blake2s.blake2s test2_plaintext_len test2_plaintext test2_key test2_key_len test2_expected_len test2_result; *)
-
-  (* Display the result *)
-  (* Lib.Print.print_compare_display test2_expected_len test2_result test2_expected; *)
-
+  C.String.print (C.String.of_literal "\nTEST 1. \n");
+  recall test1_plaintext;
+  recall test1_key;
+  recall test1_expected;
+  test_blake2s test1_size_plaintext test1_plaintext test1_size_key test1_key test1_size_expected test1_expected;
   C.EXIT_SUCCESS
